LwRust/Paper.lean
@@ -1,7 +1,4 @@
-import LwRust.Paper.BorrowChecker
+import LwRust.Paper.Syntax
 import LwRust.Paper.Runtime
 import LwRust.Paper.InductiveSemantics
-import LwRust.Paper.StoreTyping
-import LwRust.Paper.Progress
-import LwRust.Paper.Preservation
-import LwRust.Paper.Soundness
+import LwRust.Paper.Typing
